prove basic cases

Spacetalk/SimpleArith.lean
@@ -3,14 +3,80 @@ import Mathlib.Data.Vector3
 import Mathlib.Tactic.SimpRw
 import Aesop
 
-def Vector.nil_append : ∀ vNil : Vector α 0, ∀ v : Vector α n, vNil.append v = v.cast (Nat.zero_add n).symm := by
+theorem Vector.cast_toArray {h : arr.size = n} {heq : n = m} : (heq ▸ ⟨arr, h⟩ : Vector α m).toArray = arr := by
+  subst h heq
+  simp_all only
+
+def Vector.nil_append : ∀ vNil : Vector α 0, ∀ v : Vector α n, vNil.append v = (Nat.zero_add n).symm ▸ v := by
   intro vNil v
-  simp only [Vector.append, mk_eq, toArray_cast, Array.append_left_eq_self, toArray_eq_empty_iff]
+  obtain ⟨_, h_size⟩ := vNil
+  simp_rw [Array.size_eq_zero_iff.mp h_size]
+  simp only [append, Array.empty_append, mk_eq]
+  rw [Vector.cast_toArray]
 
 def Vector.split (v : Vector α (n + m)) : Vector α n × Vector α m :=
   have h_min_eq : min n (n + m) = n := Nat.min_add_right
   have h_minus_eq : n + m - n = m := by omega
-  (h_min_eq ▸ (v.take n), h_minus_eq ▸ (v.drop n))
+  (h_min_eq ▸ v.take n, h_minus_eq ▸ v.drop n)
+
+theorem Vector.plus_eq_append
+  : ∀ v : Vector α (n + m), ∃ (v1 : Vector α n) (v2 : Vector α m), v = v1.append v2 := by
+  intro v
+  have h_min_eq : min n (n + m) = n := Nat.min_add_right
+  have h_minus_eq : n + m - n = m := by omega
+  exists (h_min_eq ▸ v.take n)
+  exists (h_minus_eq ▸ v.drop n)
+  obtain ⟨arr, h⟩ := v
+  simp only [append, take_eq_extract, extract_mk, Nat.sub_zero, cast_toArray, drop_eq_cast_extract,
+    cast_mk, Array.extract_append_extract, Nat.zero_le, inf_of_le_left, Nat.le_add_right,
+    sup_of_le_right, eq_mk]
+  simp_all only [Nat.le_add_right, inf_of_le_left, Nat.add_sub_cancel_left]
+  ext i hi₁ hi₂ : 1
+  · simp_all only [Array.size_extract, min_self, Nat.sub_zero]
+  · simp_all only [Array.getElem_extract, Nat.zero_add]
+
+theorem Vector.append_split_left_eq {v1 : Vector α n} {v2 : Vector α m} : (v1.append v2).split.1 = v1 := by
+  obtain ⟨arr1, h1⟩ := v1
+  simp only [split, append, take_eq_extract, extract_mk, Nat.sub_zero, Array.extract_append,
+    Nat.zero_le, Nat.sub_eq_zero_of_le, drop_eq_cast_extract, cast_mk, eq_mk]
+  rw [Vector.cast_toArray]
+  subst h1
+  simp_all only [Array.extract_size, Nat.sub_self, Array.append_right_eq_self, Array.extract_eq_empty_iff,
+    size_toArray, Nat.zero_le, inf_of_le_left, le_refl]
+
+theorem Vector.append_split_right_eq {v1 : Vector α n} {v2 : Vector α m} : (v1.append v2).split.2 = v2 := by
+  obtain ⟨arr2, h2⟩ := v2
+  simp only [split, append, take_eq_extract, extract_mk, Nat.sub_zero, Array.extract_append,
+    Nat.zero_le, Nat.sub_eq_zero_of_le, drop_eq_cast_extract, cast_mk, eq_mk]
+  rw [Vector.cast_toArray]
+  subst h2
+  simp_all only [size_toArray, Nat.sub_self, Nat.add_sub_cancel_left, Array.extract_size, Array.append_left_eq_self,
+    Array.extract_eq_empty_iff, Nat.le_add_right, inf_of_le_right, le_refl]
+
+theorem Vector.append_split_map_left_eq {v1 : Vector α n} {v2 : Vector α m} {f : α → β}
+  : ((v1.append v2).map f).split.1 = v1.map f := by
+  obtain ⟨arr1, h1⟩ := v1
+  subst h1
+  simp only [split, append, map_mk, Array.map_append, take_eq_extract, extract_mk, Nat.sub_zero,
+    Array.extract_append, Array.size_map, Nat.zero_le, Nat.sub_eq_zero_of_le, Nat.sub_self,
+    drop_eq_cast_extract, Nat.add_sub_cancel_left, cast_mk, eq_mk, cast_toArray]
+  rw [Array.map_extract.symm]
+  simp only [Array.extract_size, Array.append_right_eq_self, Array.extract_eq_empty_iff,
+    Array.size_map, size_toArray, Nat.zero_le, inf_of_le_left, le_refl]
+
+theorem Vector.append_split_map_right_eq {v1 : Vector α n} {v2 : Vector α m} {f : α → β}
+  : ((v1.append v2).map f).split.2 = v2.map f := by
+  obtain ⟨arr1, h1⟩ := v1
+  subst h1
+  obtain ⟨arr2, h2⟩ := v2
+  subst h2
+  simp only [split, append, map_mk, Array.map_append, take_eq_extract, extract_mk, Nat.sub_zero,
+    Array.extract_append, Array.size_map, Nat.zero_le, Nat.sub_eq_zero_of_le, Nat.sub_self,
+    drop_eq_cast_extract, Nat.add_sub_cancel_left, cast_mk, eq_mk, cast_toArray]
+  rw [Array.map_extract.symm]
+  simp only [Array.extract_size_left, List.map_toArray, List.map_nil, Array.empty_append,
+    Array.extract_eq_self_iff, Array.size_map, List.length_eq_zero_iff, Array.toList_eq_nil_iff,
+    le_refl, and_self, or_true]
 
 inductive Exp : Nat → Type
   | val : Nat → Exp 0
@@ -63,8 +129,8 @@ def Exp.compileC (cont : α → Graph α nCont) : Exp nExp → Graph α (nExp + 
      e2.compileC λ e2Out =>
      .μClosed .plus #v[e1Out, e2Out] cont)
 
-theorem graph_subst {n m : Nat} {h : n = m} {g1 : Graph (Stream' Nat) n}
-  : (h ▸ g1).denote = h ▸ g1.denote := by
+theorem graph_cast_denote {n m : Nat} {h : n = m} {g1 : Graph (Stream' Nat) n} {inp : Vector (Stream' Nat) m}
+  : (h ▸ g1).denote inp = g1.denote (h ▸ inp) := by
   subst h
   simp_all only
 
@@ -78,38 +144,25 @@ theorem compileC_correct
   intro e f vInpExp vInpCont
   induction e generalizing f with
   | val v =>
-    funext i
-    simp only [Exp.denote, Stream'.const, Exp.eval, Exp.compileC, Graph.denote, Node.denote,
-      Vector.getElem_mk, List.getElem_toArray, List.getElem_cons_zero]
-    rw [Eq.rec_eq_cast]
-    -- induction nCont with
-    -- | zero =>
-    --   cases congr_arg (Graph (Stream' ℕ)) Exp.compileC.proof_6
-    --   simp [Graph.denote, Node.denote]
-    --   unfold Exp.denote
-    --   simp [Exp.eval]
-    --   unfold Stream'.const
-    --   cases vInpCont
-    --   cases vInpExp
-    --   simp [Vector.append]
-    --   rename_i heq
-    --   simp_rw [Array.size_eq_zero_iff.mp heq]
-    --   simp_rw [Array.empty_append]
-    -- | succ n ih =>
-    -- cases (congr_arg (Graph (Stream' ℕ)) Exp.compileC.proof_6)
-    cases h : Graph.μClosed (Node.val v) #v[] f
-    · contradiction
-    · rename_i node inpVec cont
-      rw [Vector.nil_append vInpExp vInpCont]
-      -- cases Eq.symm (Nat.zero_add nCont)
-      -- cases congr_arg (Graph (Stream' ℕ)) Exp.compileC.proof_6
-      -- have : 0 + nCont = nCont := by aesop
-      -- rw [this]
-      -- cases @cast (Graph (Stream' ℕ) nCont) (Graph (Stream' ℕ) (0 + nCont)) (congr_arg (Graph (Stream' ℕ)) Exp.compileC.proof_6) (Graph.μClosed node inpVec cont)
-      sorry
-    · contradiction
-
-  | var => sorry
+    -- Get rid of all castings first
+    simp only [Exp.compileC, graph_cast_denote]
+    conv =>
+      rhs
+      arg 2
+      simp only [Vector.nil_append, Eq.rec_eq_cast, cast_cast, cast_eq]
+    -- rfl closes the goal now
+    rfl
+  | var =>
+    unfold Exp.denote
+    simp only [Exp.eval, Vector.packStreams, Vector.getElem_map, Exp.compileC, Graph.denote,
+      Node.denote, Vector.append_split_left_eq, Vector.append_split_right_eq]
+    rfl
   | plus e1 e2 ih1 ih2 =>
-    simp only [Exp.denote, Exp.eval, Exp.compile, Stream'.const, Exp.compileC]
+    simp only [Exp.compileC, graph_cast_denote]
+    obtain ⟨vInp1, vInp2, h_inp⟩ := Vector.plus_eq_append vInpExp
+    rw [h_inp]
+    unfold Exp.denote
+    simp only [Exp.eval, Vector.packStreams, Vector.append_split_map_left_eq,
+      Vector.append_split_map_right_eq]
+
     sorry
